# Solution

```regex
^(x+)(x+)-\2=\1$
^(.*)(.*)(.*)=\1\3\2$
\((x+)\1*,\1*\)=\1$
^([0369]|[258][0369]*[147]|([147]|[258][0369]*[258])([0369]|[147][0369]*[258])*([258]|[147][0369]*[147]))*$
^((?=(x*).*(?=x{4}(x{5}(\2{5}))(?=\3*$)\4+$)(|x{4})(?=xx(x*)(\6x?))\5(x(x*))(?=(\8*)\9+$)(?=\8*$\10)\8*(?=(x\2\9+$))(x*)\12)\7\11(\6\11\12)|x{0,3}|x{5}|x{8}|x{21})$ (?# Theoretical solution but too slow
^(x|xx|xxx|x{5}|x{8}|x{13}|x{21}|x{34}|x{55}|x{89}|x{144}|x{233}|x{377}|x{610}|x{987}|x{1597}|x{2584}|x{4181}|x{6765})$
```